src/crypto/aes/GHash_i.fst
@@ -2,8 +2,11 @@ module GHash_i
 
 open Words_s
 open Types_s
+open Types_i
 open GHash_s
 open GF128_s
+open GCTR_s
+open GCM_helpers_i
 open Collections.Seqs_s
 open Collections.Seqs_i
 open FStar.Seq
@@ -90,3 +93,52 @@ let lemma_hash_append3 (h y_init y_mid1 y_mid2 y_final:quad32) (s1 s2 s3:seq qua
     ghash_incremental_to_ghash h s123;
     ()
   )
+
+open FStar.Mul
+let lemma_ghash_incremental_bytes_extra_helper (h y_init y_mid y_final:quad32) (input:seq quad32) (final final_padded:quad32) (num_bytes:nat) : Lemma
+  (requires (1 <= num_bytes /\ 
+             num_bytes < 16 * length input /\
+             16 * (length input - 1) < num_bytes /\
+             num_bytes % 16 <> 0 /\ //4096 * num_bytes < pow2_32 /\
+             (let num_blocks = num_bytes / 16 in
+              let full_blocks = slice_work_around input num_blocks in
+              y_mid = ghash_incremental0 h y_init full_blocks /\
+              final == index input num_blocks /\
+              (let padded_bytes = pad_to_128_bits (slice_work_around (le_quad32_to_bytes final) (num_bytes % 16)) in
+               length padded_bytes == 16 /\
+               final_padded == le_bytes_to_quad32 padded_bytes /\
+               y_final = ghash_incremental h y_mid (create 1 final_padded)))))
+  (ensures (let input_bytes = slice_work_around (le_seq_quad32_to_bytes input) num_bytes in
+            let padded_bytes = pad_to_128_bits input_bytes in
+            let input_quads = le_bytes_to_seq_quad32 padded_bytes in
+            y_final == ghash_incremental h y_init input_quads))
+  =
+  // Precondition definitions
+  let num_blocks = num_bytes / 16 in
+  let full_blocks = slice_work_around input num_blocks in
+  let padded_bytes = pad_to_128_bits (slice_work_around (le_quad32_to_bytes final) (num_bytes % 16)) in
+
+  // Postcondition definitions
+  let input_bytes = slice_work_around (le_seq_quad32_to_bytes input) num_bytes in
+  let padded_bytes' = pad_to_128_bits input_bytes in
+  let input_quads = le_bytes_to_seq_quad32 padded_bytes' in
+
+  lemma_hash_append2 h y_init y_mid y_final full_blocks final_padded;
+  assert (y_final == ghash_incremental h y_init (full_blocks @| (create 1 final_padded)));
+
+  //// Need to show that input_quads == full_blocks @| (create 1 final_padded)
+
+  // First show that the inputs to input_quads corresponds
+  pad_to_128_bits_le_quad32_to_bytes input num_bytes;
+  assert (padded_bytes' == le_seq_quad32_to_bytes (slice input 0 num_blocks) @| pad_to_128_bits (slice (le_quad32_to_bytes final) 0 (num_bytes % 16)));
+  assert (padded_bytes' == le_seq_quad32_to_bytes full_blocks @| padded_bytes);
+
+  // Start deconstructing input_quads
+  append_commutes_le_bytes_to_seq_quad32 (le_seq_quad32_to_bytes full_blocks) padded_bytes; // Distribute the le_bytes_to_seq_quad32
+  assert (input_quads == (le_bytes_to_seq_quad32 (le_seq_quad32_to_bytes full_blocks)) @| (le_bytes_to_seq_quad32 padded_bytes));
+  le_bytes_to_seq_quad32_to_bytes (slice_work_around input num_blocks);
+  assert (input_quads == full_blocks @| (le_bytes_to_seq_quad32 padded_bytes));
+  le_bytes_to_seq_quad_of_singleton final_padded padded_bytes;
+  assert (input_quads == full_blocks @| (create 1 final_padded));
+  
+  ()
